dregg-lean-ffi/src/lean_init_st.cpp
@@ -102,7 +102,7 @@ lean_object *initialize_Dregg2_Dregg2_Games_PathOfAngels_NetworkGenesis(uint8_t 
 #ifdef DREGG_POA_DARK_BAZAAR_JUDGE
 lean_object *initialize_Dregg2_Dregg2_Games_PathOfAngels_DarkBazaarJudge(uint8_t builtin);
 #endif
-#if defined(DREGG_POA_GALLEY_DAILY_JUDGE) || defined(DREGG_POA_GALLEY_DAILY_SPONSOR_JUDGE)
+#ifdef DREGG_POA_GALLEY_DAILY_JUDGE
 lean_object *initialize_Dregg2_Dregg2_Games_PathOfAngels_GalleyMaintenanceDailyRuntime(uint8_t builtin);
 #endif
 #if defined(DREGG_POA_EVENT_BATCH_RUNTIME_PLAN) || \
@@ -206,7 +206,7 @@ extern "C" int dregg_ffi_init_st(void) {
         lean_dec_ref(bazaarres);
     }
 #endif
-#if defined(DREGG_POA_GALLEY_DAILY_JUDGE) || defined(DREGG_POA_GALLEY_DAILY_SPONSOR_JUDGE)
+#ifdef DREGG_POA_GALLEY_DAILY_JUDGE
     {
         lean_object *galleyres =
             initialize_Dregg2_Dregg2_Games_PathOfAngels_GalleyMaintenanceDailyRuntime(1);
